src/program_proof/tulip/invariance/local_read.v
@@ -1,0 +1,209 @@
+From Perennial.program_proof.tulip Require Import prelude.
+
+Section local_read.
+  Context `{!tulip_ghostG Σ}.
+
+  Lemma replica_inv_local_read γ gid rid key rts spts pts hist :
+    key ∈ keys_all ->
+    (pts = O ∨ rts ≤ pts)%nat ->
+    own_dura_hist_half γ rid key hist -∗
+    own_replica_pts_half γ rid key pts -∗
+    own_replica_spts_half γ rid key spts -∗
+    replica_inv γ gid rid ==∗
+    own_dura_hist_half γ rid key hist ∗
+    own_replica_pts_half γ rid key pts ∗
+    own_replica_spts_half γ rid key (spts `max` rts)%nat ∗
+    replica_inv γ gid rid ∗
+    read_promise γ gid rid key (pred (length hist)) rts ∗
+    is_repl_hist_lb γ key hist.
+  Proof.
+    iIntros (Hkey Hlock) "Hhist Hpts Hspts Hrp".
+    do 2 iNamed "Hrp".
+    pose proof (apply_cmds_dom _ _ _ Hrsm) as Hdomhistm.
+    pose proof (map_Forall2_dom_L _ _ _ Hlenkvd) as Hdomsptsm.
+    symmetry in Hdomsptsm. rewrite Hdomkvdm in Hdomsptsm.
+    pose proof (map_Forall2_dom_L _ _ _ Hsptsmlk) as Hdomptsm.
+    symmetry in Hdomptsm. rewrite Hdomsptsm in Hdomptsm.
+    assert (is_Some (histm !! key)) as [hist' Hhist]; first by rewrite -elem_of_dom Hdomhistm.
+    assert (is_Some (kvdm !! key)) as [vd Hvd]; first by rewrite -elem_of_dom Hdomkvdm.
+    assert (is_Some (sptsm !! key)) as [spts' Hspts]; first by rewrite -elem_of_dom Hdomsptsm.
+    assert (is_Some (ptsm !! key)) as [pts' Hpts]; first by rewrite -elem_of_dom Hdomptsm.
+    pose proof (map_Forall2_lookup_Some _ _ _ _ _ _ Hvd Hspts Hlenkvd) as Hlenvd.
+    simpl in Hlenvd.
+    iDestruct (big_sepM_lookup_acc with "Hhistm") as "[Hhistr HhistmC]"; first apply Hhist.
+    iDestruct (big_sepM_delete with "Hkvdm") as "[Hkvd Hkvdm]"; first apply Hvd.
+    iDestruct (big_sepM_delete with "Hsptsm") as "[Hsptsr Hsptsm]"; first apply Hspts.
+    iDestruct (big_sepM_lookup_acc with "Hptsm") as "[Hptsr HptsmC]"; first apply Hpts.
+    (* Agree on the history, prepare ts, and smallest preparable ts of [key]. *)
+    iDestruct (dura_hist_agree with "Hhist Hhistr") as %->.
+    iDestruct (replica_spts_agree with "Hspts Hsptsr") as %->.
+    iDestruct (replica_pts_agree with "Hpts Hptsr") as %->.
+    destruct (decide (pts = O)) as [Hz | Hnz]; last first.
+    { (* Case: Key locked by txn [pts] where [rts ≤ pts]. No extension required. *)
+      destruct Hlock as [? | Hle]; first done.
+      pose proof (map_Forall2_lookup_Some _ _ _ _ _ _ Hspts Hpts Hsptsmlk Hnz) as Hsptslk.
+      iAssert (read_promise γ gid rid key (pred (length hist)) rts)%I as "#Hpromise".
+      { iDestruct (replica_key_validation_witness with "Hkvd") as "#Hkvdlb".
+        iDestruct (replica_key_validation_lb_weaken (take rts vd) with "Hkvdlb") as "#Hlb".
+        { apply prefix_take. }
+        iFrame "Hlb".
+        iSplit; last first.
+        { iPureIntro.
+          rewrite length_take.
+          clear -Hlenvd Hsptslk Hle. lia.
+        }
+        iApply big_sepL_forall.
+        iIntros (t b Hb [Htge ->]).
+        assert (Hvdtrue : vd !! t = Some true).
+        { eapply prefix_lookup_Some; first apply Hb.
+          apply prefix_take.
+        }
+        iSpecialize ("Hgabt" $! key t).
+        rewrite Hvd Hhist Hpts Hvdtrue.
+        case_decide as Ht; first iFrame "Hgabt".
+        exfalso.
+        apply Classical_Prop.not_and_or in Ht.
+        destruct Ht as [Htlt | Hnpt].
+        { clear -Htlt Htge. lia. }
+        apply dec_stable in Hnpt. subst t.
+        apply lookup_lt_Some in Hb.
+        rewrite length_take_le in Hb; last first.
+        { clear -Hle Hlenvd Hsptslk. lia. }
+        clear -Hb Hle. lia.
+      }
+      replace (_ `max` _)%nat with spts by lia.
+      iDestruct ("HhistmC" with "Hhistr") as "Hhistm".
+      iDestruct (big_sepM_insert_2 with "Hkvd Hkvdm") as "Hkvdm".
+      rewrite insert_delete; last apply Hvd.
+      iDestruct (big_sepM_insert_2 with "Hsptsr Hsptsm") as "Hsptsm".
+      rewrite insert_delete; last apply Hspts.
+      iDestruct ("HptsmC" with "Hptsr") as "Hptsm".
+      (* Obtain a lower-bound on the replicated history. *)
+      iDestruct (big_sepM_lookup with "Hreplhm") as "Hreplh"; first apply Hhist.
+      by iFrame "∗ # %".
+    }
+    (* Case: Key not locked. *)
+    destruct (decide (rts ≤ spts)%nat) as [Hle | Hgt].
+    { (* Case: [rts ≤ spts]. No extension required. *)
+      iAssert (read_promise γ gid rid key (pred (length hist)) rts)%I as "#Hpromise".
+      { iDestruct (replica_key_validation_witness with "Hkvd") as "#Hkvdlb".
+        iDestruct (replica_key_validation_lb_weaken (take rts vd) with "Hkvdlb") as "#Hlb".
+        { apply prefix_take. }
+        iFrame "Hlb".
+        iSplit; last first.
+        { iPureIntro.
+          rewrite length_take.
+          clear -Hlenvd Hle. lia.
+        }
+        iApply big_sepL_forall.
+        iIntros (t b Hb [Htge ->]).
+        assert (Hvdtrue : vd !! t = Some true).
+        { eapply prefix_lookup_Some; first apply Hb.
+          apply prefix_take.
+        }
+        iSpecialize ("Hgabt" $! key t).
+        rewrite Hvd Hhist Hpts Hvdtrue.
+        case_decide as Ht; first iFrame "Hgabt".
+        exfalso.
+        clear -Ht Htge Hz. lia.
+      }
+      replace (_ `max` _)%nat with spts by lia.
+      iDestruct ("HhistmC" with "Hhistr") as "Hhistm".
+      iDestruct (big_sepM_insert_2 with "Hkvd Hkvdm") as "Hkvdm".
+      rewrite insert_delete; last apply Hvd.
+      iDestruct (big_sepM_insert_2 with "Hsptsr Hsptsm") as "Hsptsm".
+      rewrite insert_delete; last apply Hspts.
+      iDestruct ("HptsmC" with "Hptsr") as "Hptsm".
+      (* Obtain a lower-bound on the replicated history. *)
+      iDestruct (big_sepM_lookup with "Hreplhm") as "Hreplh"; first apply Hhist.
+      by iFrame "∗ # %".
+    }
+    (* Case: [spts < rts]. Extend the key validation list with [false] until
+    [rts] and update the smallest ts to [rts]. *)
+    rewrite Nat.nle_gt in Hgt.
+    set vd' := extend rts false vd.
+    iMod (replica_key_validation_update vd' with "Hkvd") as "Hkvd".
+    { apply extend_prefix. }
+    iMod (replica_spts_update rts with "Hspts Hsptsr") as "[Hspts Hsptsr]".
+    replace (_ `max` _)%nat with rts by lia.
+    iAssert (read_promise γ gid rid key (pred (length hist)) rts)%I as "#Hpromise".
+    { iDestruct (replica_key_validation_witness with "Hkvd") as "#Hkvdlb".
+      iFrame "Hkvdlb".
+      iSplit; last first.
+      { iPureIntro. rewrite extend_length. clear -Hlenvd Hgt. lia. }
+      iApply big_sepL_forall.
+      iIntros (t b Hb [Htge ->]).
+      destruct (decide (t < spts)%nat) as [Hlt | Hge].
+      { rewrite lookup_extend_l in Hb; last first.
+        { clear -Hlenvd Hlt. lia. }
+        iSpecialize ("Hgabt" $! key t).
+        rewrite Hvd Hhist Hpts Hb.
+        case_decide as Ht; first iFrame "Hgabt".
+        exfalso.
+        clear -Ht Htge Hz. lia.
+      }
+      exfalso.
+      rewrite Nat.nlt_ge in Hge.
+      apply lookup_lt_Some in Hb as Htlt.
+      rewrite extend_length in Htlt.
+      rewrite lookup_extend_r in Hb; first done.
+      clear -Hlenvd Hgt Hge Htlt. lia.
+    }
+    iDestruct ("HhistmC" with "Hhistr") as "Hhistm".
+    iDestruct (big_sepM_insert_2 with "Hkvd Hkvdm") as "Hkvdm".
+    rewrite insert_delete_insert.
+    iDestruct (big_sepM_insert_2 with "Hsptsr Hsptsm") as "Hsptsm".
+    rewrite insert_delete_insert.
+    iDestruct ("HptsmC" with "Hptsr") as "Hptsm".
+    (* Obtain a lower-bound on the replicated history. *)
+    iDestruct (big_sepM_lookup with "Hreplhm") as "Hreplh"; first apply Hhist.
+    iFrame "∗ # %".
+    iModIntro.
+    iSplit.
+    { iIntros (k t).
+      destruct (decide (k = key)) as [-> | Hne]; last first.
+      { by rewrite lookup_insert_ne. }
+      rewrite lookup_insert Hhist Hpts.
+      destruct (decide (rts ≤ t)%nat) as [Hgerts | Hltrts].
+      { rewrite lookup_ge_None_2; first done.
+        rewrite extend_length.
+        clear -Hlenvd Hgerts Hgt. lia.
+      }
+      rewrite Nat.nle_gt in Hltrts.
+      destruct (decide (t < spts)%nat) as [Hltspts | Hgespts]; last first.
+      { rewrite Nat.nlt_ge in Hgespts.
+        rewrite lookup_extend_r; first done.
+        clear -Hlenvd Hltrts Hgespts. lia.
+      }
+      rewrite lookup_extend_l; last first.
+      { clear -Hlenvd Hltspts. lia. }
+      iSpecialize ("Hgabt" $! key t).
+      by rewrite Hvd Hhist Hpts.
+    }
+    iPureIntro.
+    split.
+    { rewrite dom_insert_L.
+      clear -Hkey Hdomkvdm. set_solver.
+    }
+    split.
+    { apply map_Forall2_insert_2; last apply Hlenkvd.
+      rewrite extend_length.
+      clear -Hlenvd Hgt. lia.
+    }
+    { rewrite map_Forall2_forall.
+      split; last first.
+      { rewrite dom_insert_L. clear -Hkey Hdomsptsm Hdomptsm. set_solver. }
+      intros k sptsx ptsx Hsptsx Hptsx Hnz.
+      destruct (decide (k = key)) as [-> | Hne]; last first.
+      { rewrite lookup_insert_ne in Hsptsx; last done.
+        rewrite map_Forall2_forall in Hsptsmlk.
+        destruct Hsptsmlk as [Hsptsmlk _].
+        by eapply Hsptsmlk.
+      }
+      exfalso.
+      rewrite Hpts in Hptsx.
+      clear -Hz Hnz Hptsx. inv Hptsx.
+    }
+  Qed.
+
+End local_read.
